compiler/yul/Owned.yul
@@ -15,6 +15,9 @@ object "Owned" {
                 if callvalue() {
                     revert(0, 0)
                 }
+                if lt(calldatasize(), 36) {
+                    revert(0, 0)
+                }
                 let newOwner := and(calldataload(4), 0xffffffffffffffffffffffffffffffffffffffff)
                 if iszero(eq(caller(), sload(0))) {
                     mstore(0, 0x8c379a000000000000000000000000000000000000000000000000000000000)
@@ -29,6 +32,9 @@ object "Owned" {
             case 0x893d20e8 {
                 /* getOwner() */
                 if callvalue() {
+                    revert(0, 0)
+                }
+                if lt(calldatasize(), 4) {
                     revert(0, 0)
                 }
                 mstore(0, sload(0))
