compiler/yul/SafeCounter.yul
@@ -11,6 +11,9 @@ object "SafeCounter" {
                 if callvalue() {
                     revert(0, 0)
                 }
+                if lt(calldatasize(), 4) {
+                    revert(0, 0)
+                }
                 let count := sload(0)
                 let newCount := add(count, 1)
                 if iszero(gt(newCount, count)) {
@@ -28,6 +31,9 @@ object "SafeCounter" {
                 if callvalue() {
                     revert(0, 0)
                 }
+                if lt(calldatasize(), 4) {
+                    revert(0, 0)
+                }
                 let count := sload(0)
                 if lt(count, 1) {
                     mstore(0, 0x8c379a000000000000000000000000000000000000000000000000000000000)
@@ -42,6 +48,9 @@ object "SafeCounter" {
             case 0xa87d942c {
                 /* getCount() */
                 if callvalue() {
+                    revert(0, 0)
+                }
+                if lt(calldatasize(), 4) {
                     revert(0, 0)
                 }
                 mstore(0, sload(0))
